Utils.thy
@@ -24,31 +24,17 @@ lemma fresh_star_empty[simp]: "{} \<sharp>* x" by (simp add: fresh_star_def)
 
 section\<open>Headers\<close>
 
-text\<open>This is necessary to use headers (and heaps later)  in nominal_functions. It basically states
-that no variables actually appear in the type.\<close>
-instantiation headers :: pure begin
-  definition permute_headers :: "perm \<Rightarrow> headers \<Rightarrow> headers" where
-    "permute_headers _ x = x"
-  instance by standard (auto simp add: permute_headers_def)
-end
-
-definition "empty_headers = Headers Map.empty"
-
-fun header_lookup :: "headers \<Rightarrow> instanc \<Rightarrow> bv option" where
-  "header_lookup (Headers h) i = h i" 
-
-fun header_update :: "headers \<Rightarrow> instanc \<Rightarrow> bv \<Rightarrow> headers" where
-  "header_update (Headers h) i bs = Headers (h(i := Some bs))"
+definition empty_headers :: headers where "empty_headers = Map.empty"
 
 fun header_field_to_range_helper :: "nat \<Rightarrow> field list \<Rightarrow> field_name \<Rightarrow> (nat \<times> nat)" where
-  "header_field_to_range_helper acc ((Field fn fl)#fs) tgt = (if fn = tgt then (acc, acc + fl)
-    else header_field_to_range_helper (acc + fl) fs tgt)" |
+  "header_field_to_range_helper acc (f#fs) tgt = (if field_name f = tgt then (acc, acc + field_length f)
+    else header_field_to_range_helper (acc + field_length f) fs tgt)" |
   "header_field_to_range_helper acc [] tgt = undefined"
 
 fun header_field_to_range :: "header_type \<Rightarrow> field_name \<Rightarrow> (nat \<times> nat)" where
-  "header_field_to_range (HeaderType _ fs) tgt = header_field_to_range_helper 0 fs tgt"
+  "header_field_to_range \<eta> tgt = header_field_to_range_helper 0 (header_fields \<eta>) tgt"
 lemma header_field_to_range_eqvt[eqvt]:
-  "p \<bullet> header_field_to_range ht f = header_field_to_range (p \<bullet> ht) (p \<bullet> f)"
+  "p \<bullet> header_field_to_range \<eta> f = header_field_to_range (p \<bullet> \<eta>) (p \<bullet> f)"
   by (simp add: permute_pure)
 
 fun field_list_to_range :: "field list \<Rightarrow> field_name \<Rightarrow> (nat \<times> nat)" where
@@ -57,84 +43,75 @@ lemma field_list_to_range_eqvt[eqvt]:
   "p \<bullet> field_list_to_range fs tgt = field_list_to_range (p \<bullet> fs) (p \<bullet> tgt)"
   by (simp add: permute_pure)
 
-fun header_length :: "header_type \<Rightarrow> nat" where
-  "header_length (HeaderType _ fs) = (\<Sum>f\<leftarrow>fs. case f of field.Field x fl \<Rightarrow> fl)"
-
+definition header_length :: "header_type \<Rightarrow> nat" where
+  "header_length ht = (\<Sum>f \<leftarrow> header_fields ht. field_length f)"
 lemma header_length_eqvt[eqvt]: "p \<bullet> header_length ht = header_length (p \<bullet> ht)"
   by (auto simp add: permute_pure)
 
-fun init_header :: "header_type \<Rightarrow> bv" where
+definition init_header :: "header_type \<Rightarrow> bv" where
   "init_header \<eta> = replicate (header_length \<eta>) False"
 
-fun serialize_header :: "headers \<Rightarrow> instanc \<Rightarrow> bv option" where
-  "serialize_header (Headers h) i = h i"
+definition serialize_header :: "headers \<Rightarrow> instanc \<Rightarrow> bv option" where
+  "serialize_header H i = H i"
 
-fun deserialize_header :: "header_type \<Rightarrow> bv \<Rightarrow> (bv \<times> bv)" where
+definition deserialize_header :: "header_type \<Rightarrow> bv \<Rightarrow> (bv \<times> bv)" where
   "deserialize_header \<eta> In = (let len = header_length \<eta> in (take len In, drop len In))"
 
-fun join_headers :: "headers \<Rightarrow> headers \<Rightarrow> headers" where
-  "join_headers (Headers h\<^sub>1) (Headers h\<^sub>2) = Headers (Map.map_add h\<^sub>1 h\<^sub>2)"
+definition join_headers :: "headers \<Rightarrow> headers \<Rightarrow> headers" where
+  "join_headers H\<^sub>1 H\<^sub>2 = (Map.map_add H\<^sub>1 H\<^sub>2)"
 
 section\<open>Heaps\<close>
 
-instantiation heap :: pure begin
-  definition permute_heap :: "perm \<Rightarrow> heap \<Rightarrow> heap"  where
-    "permute_heap _ x = x"
-  instance by standard (auto simp add: permute_heap_def)
-end
-
-fun triple_to_heap :: "bv \<Rightarrow> bv \<Rightarrow> headers \<Rightarrow> heap" where
-  "triple_to_heap In Out H = Heap In Out H"
-
-fun heap_dom :: "heap \<Rightarrow> instanc set" where
-  "heap_dom (Heap _ _ (Headers H)) = dom H"
+definition heap_dom :: "heap \<Rightarrow> instanc set" where
+  "heap_dom h = dom (heap_headers h)"
 
 fun heap_lookup_packet :: "heap \<Rightarrow> packet \<Rightarrow> bv" where
-  "heap_lookup_packet (Heap In Out _) PktIn = In" |
-  "heap_lookup_packet (Heap In Out _) PktOut = Out"
-
+  "heap_lookup_packet h PktIn = heap_pkt_in h" |
+  "heap_lookup_packet h PktOut = heap_pkt_out h"
 lemma heap_lookup_packet_eqvt[eqvt]:
   "p \<bullet> heap_lookup_packet h pkt = heap_lookup_packet (p \<bullet> h) (p \<bullet> pkt)"
   by (simp add: permute_pure)
 
 fun heap_lookup_instance :: "heap \<Rightarrow> instanc \<Rightarrow> bv option" where
-  "heap_lookup_instance (Heap _ _ (Headers insts)) i = insts i"
-
+  "heap_lookup_instance h \<iota> = (heap_headers h) \<iota>"
 lemma heap_lookup_instance_eqvt[eqvt]:
-  "p \<bullet> heap_lookup_instance h i = heap_lookup_instance (p \<bullet> h) (p \<bullet> i)"
+  "p \<bullet> heap_lookup_instance h \<iota> = heap_lookup_instance (p \<bullet> h) (p \<bullet> \<iota>)"
   by (simp add: permute_pure)
 
 no_notation map_add (infixl "++" 100) \<comment> \<open>avoid clash with built-in map_add notation\<close>
-fun concat_heaps :: "heap \<Rightarrow> heap \<Rightarrow> heap" (infixl "++" 100) where
-  "concat_heaps (Heap In\<^sub>1 Out\<^sub>1 H\<^sub>1) (Heap In\<^sub>2 Out\<^sub>2 H\<^sub>2)
-    = Heap (In\<^sub>1 @ In\<^sub>2) (Out\<^sub>1 @ Out\<^sub>2) (join_headers H\<^sub>1 H\<^sub>2)"
-
+definition concat_heaps :: "heap \<Rightarrow> heap \<Rightarrow> heap" (infixl "++" 100) where
+  "concat_heaps h\<^sub>1 h\<^sub>2
+    = \<lparr>heap_pkt_in = heap_pkt_in h\<^sub>1 @ heap_pkt_in h\<^sub>2,
+       heap_pkt_out = heap_pkt_out h\<^sub>1 @ heap_pkt_out h\<^sub>2,
+       heap_headers = join_headers (heap_headers h\<^sub>1) (heap_headers h\<^sub>2)\<rparr>"
 lemma concat_heaps_eqvt[eqvt]: "p \<bullet> concat_heaps h\<^sub>1 h\<^sub>2 = concat_heaps (p \<bullet> h\<^sub>1) (p \<bullet> h\<^sub>2)"
   by (simp add: permute_pure)
 
+
 section\<open>Environments\<close>
 
-fun env_lookup_packet :: "env \<Rightarrow> var \<Rightarrow> packet \<Rightarrow> bv option" where
-  "env_lookup_packet \<epsilon> x p = map_option (\<lambda>h. heap_lookup_packet h p) (map_of \<epsilon> x)"
+definition env_lookup_packet :: "env \<Rightarrow> var \<Rightarrow> packet \<Rightarrow> bv option" where
+  "env_lookup_packet \<E> x p = map_option (\<lambda>h. heap_lookup_packet h p) (map_of \<E> x)"
 
-fun env_lookup_instance :: "env \<Rightarrow> var \<Rightarrow> instanc \<Rightarrow> bv option" where
-  "env_lookup_instance \<epsilon> x i = Option.bind (map_of \<epsilon> x) (\<lambda>h. heap_lookup_instance h i)"
+definition env_lookup_instance :: "env \<Rightarrow> var \<Rightarrow> instanc \<Rightarrow> bv option" where
+  "env_lookup_instance \<E> x \<iota> = Option.bind (map_of \<E> x) (\<lambda>h. heap_lookup_instance h \<iota>)"
 
 nominal_function env_lookup_sliceable :: "env \<Rightarrow> sliceable \<Rightarrow> bv option" where
-  "env_lookup_sliceable \<epsilon> (SlPacket x p) = env_lookup_packet \<epsilon> x p" |
-  "env_lookup_sliceable \<epsilon> (SlInstance x i) = env_lookup_instance \<epsilon> x i"
-  subgoal by (simp add: eqvt_def env_lookup_sliceable_graph_aux_def)
+  "env_lookup_sliceable \<E> (SlPacket x p) = env_lookup_packet \<E> x p" |
+  "env_lookup_sliceable \<E> (SlInstance x \<iota>) = env_lookup_instance \<E> x \<iota>"
+  subgoal by (simp add: eqvt_def env_lookup_sliceable_graph_aux_def
+                        env_lookup_packet_def env_lookup_instance_def)
   subgoal by (erule env_lookup_sliceable_graph.induct) (auto)
   apply clarify
-  subgoal for P e s
+  subgoal for P \<E> s
     by (rule sliceable.strong_exhaust[of s P]) (auto)
   apply (simp_all)
 done
 nominal_termination (eqvt)
   by lexicographic_order
 
-lemma env_update_eqvt[eqvt]: "p \<bullet> \<epsilon>[x \<rightarrow> h] = (p \<bullet> \<epsilon>)[p \<bullet> x \<rightarrow> p \<bullet> h]"
-  by (induct \<epsilon>) (auto simp add: permute_pure env_update_def)
+lemma env_update_eqvt[eqvt]: "p \<bullet> \<E>[x \<rightarrow> h] = (p \<bullet> \<E>)[p \<bullet> x \<rightarrow> p \<bullet> h]"
+  by (induct \<E>) (auto simp add: permute_pure env_update_def)
 
 section\<open>Helper for creating formulas\<close>
 
@@ -148,17 +125,17 @@ lemma mk_and_eqvt[eqvt]: "p \<bullet> mk_and \<phi>s = mk_and (p \<bullet> \<phi
 
 text\<open>Predicate for whether an entire instance is equal in the given two heaps.\<close>
 definition mk_instance_eq :: "header_type \<Rightarrow> instanc \<Rightarrow> var \<Rightarrow> var \<Rightarrow> formula" where
-  "mk_instance_eq ht i x y = (let hl = header_length ht in
-    Eq (Slice (SlInstance x i) 0 hl) (Slice (SlInstance y i) 0 hl))"
+  "mk_instance_eq \<eta> \<iota> x y = (let hl = header_length \<eta> in
+    Eq (Slice (SlInstance x \<iota>) 0 hl) (Slice (SlInstance y \<iota>) 0 hl))"
 lemma mk_instance_eq_eqvt[eqvt]:
-  "p \<bullet> mk_instance_eq ht i x y = mk_instance_eq (p \<bullet> ht) (p \<bullet> i) (p \<bullet> x) (p \<bullet> y)"
+  "p \<bullet> mk_instance_eq \<eta> \<iota> x y = mk_instance_eq (p \<bullet> \<eta>) (p \<bullet> \<iota>) (p \<bullet> x) (p \<bullet> y)"
   by (auto simp add: mk_instance_eq_def permute_pure Let_def)
 
 text\<open>Instance equality:
 Predicate for whether two heaps are equivalent in terms of all possible instances.
 Corresponds to \<equiv>_i in the paper.\<close>
 definition mk_heap_eq_instances :: "header_table \<Rightarrow> var \<Rightarrow> var \<Rightarrow> formula" where
-  "mk_heap_eq_instances HT x y = mk_and [mk_instance_eq ht i x y. (i, ht) \<leftarrow> HT]"
+  "mk_heap_eq_instances HT x y = mk_and [mk_instance_eq \<eta> \<iota> x y. (\<iota>, \<eta>) \<leftarrow> HT]"
 lemma mk_heap_eq_instances_eqvt[eqvt]:
   "p \<bullet> mk_heap_eq_instances HT x y = mk_heap_eq_instances (p \<bullet> HT) (p \<bullet> x) (p \<bullet> y)"
   by (auto simp add: mk_heap_eq_instances_def permute_pure)
@@ -176,25 +153,25 @@ lemma mk_heap_eq_eqvt[eqvt]: "p \<bullet> mk_heap_eq HT x y = mk_heap_eq (p \<bu
 text\<open>Like mk_heap_eq_instances but ignoring the given instance.\<close>
 definition mk_heap_eq_instances_except :: "header_table \<Rightarrow> instanc \<Rightarrow> var \<Rightarrow> var \<Rightarrow> formula"
 where
-  "mk_heap_eq_instances_except HT i x y = mk_heap_eq_instances [(k,ht)\<leftarrow>HT. k \<noteq> i] x y"
+  "mk_heap_eq_instances_except HT \<iota> x y = mk_heap_eq_instances [(\<kappa>,\<eta>)\<leftarrow>HT. \<kappa> \<noteq> \<iota>] x y"
 lemma mk_heap_eq_instances_except_eqvt[eqvt]:
   "p \<bullet> mk_heap_eq_instances_except HT i x y = mk_heap_eq_instances_except (p \<bullet> HT) (p \<bullet> i) (p \<bullet> x) (p \<bullet> y)"
   by (simp add: mk_heap_eq_instances_except_def permute_pure)
 
 definition mk_single_field_eq :: "header_type \<Rightarrow> instanc \<Rightarrow> field_name \<Rightarrow> var \<Rightarrow> var \<Rightarrow> formula"
 where
-  "mk_single_field_eq ht f i x y = (let (n, m) = header_field_to_range ht f in
-    Eq (Slice (SlInstance x i) n m) (Slice (SlInstance y i) n m))"
+  "mk_single_field_eq \<eta> f \<iota> x y = (let (n, m) = header_field_to_range \<eta> f in
+    Eq (Slice (SlInstance x \<iota>) n m) (Slice (SlInstance y \<iota>) n m))"
 lemma mk_single_field_eq_eqvt[eqvt]:
-  "p \<bullet> mk_single_field_eq ht f i x y = mk_single_field_eq (p \<bullet> ht) (p \<bullet> f) (p \<bullet> i) (p \<bullet> x) (p \<bullet> y)"
+  "p \<bullet> mk_single_field_eq \<eta> f \<iota> x y = mk_single_field_eq (p \<bullet> \<eta>) (p \<bullet> f) (p \<bullet> \<iota>) (p \<bullet> x) (p \<bullet> y)"
   by (simp add: mk_single_field_eq_def permute_pure)
 
 definition mk_fields_eq_except :: "header_type \<Rightarrow> instanc \<Rightarrow> field_name \<Rightarrow> var \<Rightarrow> var \<Rightarrow> formula"
 where
-  "mk_fields_eq_except ht i g x y = (case ht of HeaderType _ fs \<Rightarrow>
-    mk_and [mk_single_field_eq ht f i x y. (Field f _) \<leftarrow> fs, f \<noteq> g])"
+  "mk_fields_eq_except \<eta> \<iota> g x y =
+    mk_and [mk_single_field_eq \<eta> (field_name f) \<iota> x y. f \<leftarrow> header_fields \<eta>, field_name f \<noteq> g]"
 lemma mk_fields_eq_except_eqvt[eqvt]:
   "p \<bullet> mk_fields_eq_except ht i g x y = mk_fields_eq_except (p \<bullet> ht) (p \<bullet> i) (p \<bullet> g) (p \<bullet> x) (p \<bullet> y)"
-  sorry
+  by (simp add: mk_fields_eq_except_def permute_pure)
 
 end
